wip

Foundation/Modal/Kripke/Logic/Grz/Completeness.lean
@@ -8,7 +8,7 @@ namespace Formula
 variable {α : Type u} [DecidableEq α]
 variable {φ ψ χ : Formula ℕ}
 
-@[grind] noncomputable abbrev subformulasGrz (φ : Formula α) := φ.subformulas ∪ (φ.subformulas.prebox.image (λ ψ => □(ψ ➝ □ψ)))
+@[grind] noncomputable abbrev subformulasGrz (φ : Formula α) := φ.subformulas ∪ ((□'⁻¹φ.subformulas).image (λ ψ => □(ψ ➝ □ψ)))
 
 namespace subformulasGrz
 
@@ -16,7 +16,7 @@ namespace subformulasGrz
 
 @[grind ⇒] protected lemma mem_of_mem_subformula (h : ψ ∈ φ.subformulas) : ψ ∈ φ.subformulasGrz := by simp_all [subformulasGrz];
 
-@[grind ⇒] lemma mem_boximpbox (h : ψ ∈ φ.subformulas.prebox) : □(ψ ➝ □ψ) ∈ φ.subformulasGrz := by simp_all [subformulasGrz];
+@[grind ⇒] lemma mem_boximpbox (h : ψ ∈ (□'⁻¹φ.subformulas)) : □(ψ ➝ □ψ) ∈ φ.subformulasGrz := by simp_all [subformulasGrz];
 
 @[grind ⇒]
 protected lemma mem_imp (h : (ψ ➝ χ) ∈ φ.subformulasGrz) : ψ ∈ φ.subformulasGrz ∧ χ ∈ φ.subformulasGrz := by
@@ -50,8 +50,8 @@ variable {φ ψ : Formula ℕ}
 abbrev miniCanonicalFrame (𝓢 : S) [Entailment.Grz 𝓢] [Entailment.Consistent 𝓢] (φ : Formula ℕ) : Kripke.Frame where
   World := ComplementClosedConsistentFinset 𝓢 (φ.subformulasGrz)
   Rel X Y :=
-    (∀ ψ ∈ (φ.subformulasGrz).prebox, □ψ ∈ X → □ψ ∈ Y) ∧
-    ((∀ ψ ∈ (φ.subformulasGrz).prebox, □ψ ∈ Y → □ψ ∈ X) → X = Y)
+    (∀ ψ ∈ □'⁻¹(φ.subformulasGrz), □ψ ∈ X → □ψ ∈ Y) ∧
+    ((∀ ψ ∈ □'⁻¹(φ.subformulasGrz), □ψ ∈ Y → □ψ ∈ X) → X = Y)
 
 instance : (miniCanonicalFrame 𝓢 φ).IsReflexive where
   refl := by tauto_set;
@@ -87,15 +87,15 @@ abbrev miniCanonicalModel (𝓢 : S) [Entailment.Grz 𝓢] [Entailment.Consisten
 omit [Consistent 𝓢] [Entailment.Grz 𝓢] in
 lemma truthlemma_lemma1
   {X : ComplementClosedConsistentFinset 𝓢 (φ.subformulasGrz)} (hq : □ψ ∈ φ.subformulas)
-  : ((X.1.prebox.box) ∪ {□(ψ ➝ □ψ), -ψ}) ⊆ (φ.subformulasGrz)⁻ := by
+  : ((□'□'⁻¹X.1) ∪ {□(ψ ➝ □ψ), -ψ}) ⊆ (φ.subformulasGrz)⁻ := by
   simp only [FormulaFinset.complementary];
   intro χ hr;
   apply Finset.mem_union.mpr;
   replace hr : χ = □(ψ ➝ □ψ) ∨ χ = -ψ ∨ (∃ a, □a ∈ X ∧ □a = χ)  := by
-    simpa [Finset.mem_union] using hr;
+    simpa [Finset.mem_union, Finset.LO.preboxItr, Finset.LO.boxItr] using hr;
   rcases hr with (rfl | rfl | ⟨χ, hr, rfl⟩);
   . left;
-    simp;
+    simp [Finset.LO.preboxItr];
     tauto;
   . right;
     simp only [Finset.mem_image, Finset.mem_union, Finset.mem_preimage, Function.iterate_one];
@@ -105,44 +105,48 @@ lemma truthlemma_lemma1
     left;
     exact FormulaFinset.complementary_mem_box (by grind) this;
 
+set_option linter.style.multiGoal false in
 omit [Consistent 𝓢] in
 lemma truthlemma_lemma2
   {X : ComplementClosedConsistentFinset 𝓢 (φ.subformulasGrz)}
   (hψ₁ : □ψ ∈ φ.subformulas)
   (hψ₂ : □ψ ∉ X)
-  : FormulaFinset.Consistent 𝓢 ((X.1.prebox.box) ∪ {□(ψ ➝ □ψ), -ψ}) := by
+  : FormulaFinset.Consistent 𝓢 ((□'□'⁻¹X.1) ∪ {□(ψ ➝ □ψ), -ψ}) := by
     apply FormulaFinset.intro_union_consistent;
     rintro Γ₁ Γ₂ hΓ₁ hΓ₂;
     by_contra! hC;
     apply hψ₂;
-    have := Context.weakening! (Γ := Γ₁ ∪ Γ₂) (Δ := insert (-ψ) (insert (□(ψ ➝ □ψ)) Γ₁)) ?_ hC;
-    . replace := Context.deduct! this;
-      replace := of_imply_complement_bot this;
-      replace := Context.deduct! this;
-      replace := Context.nec! this;
-      replace := axiomGrz! ⨀ this;
-      replace := Context.nec! this;
-      replace := Context.boxbox_in_context_to_box this;
-      replace : X.1.toSet.prebox.box.box *⊢[𝓢] □ψ := Context.weakening! ?_ this;
-      . replace := Context.boxbox_in_context_to_box this;
-        replace : X *⊢[𝓢] □ψ := Context.weakening! ?_ this;
-        . exact membership_iff (subformulasGrz.mem_of_mem_subformula hψ₁) |>.mpr this;
-        . intro ξ hξ;
-          obtain ⟨ξ, hξ, rfl⟩ := hξ;
-          tauto;
-      . intro ξ hξ;
-        obtain ⟨ξ, hξ, rfl⟩ := hξ;
-        have := hΓ₁ hξ;
-        simp at this ⊢;
-        obtain ⟨χ, hχ, rfl⟩ := this;
-        use χ;
-    . intro ξ;
+    have    : insert (-ψ) (insert (□(ψ ➝ □ψ)) ↑Γ₁) *⊢[𝓢] ⊥ := Context.weakening! ?h₁ hC;
+    replace : (insert (□(ψ ➝ □ψ)) ↑Γ₁) *⊢[𝓢] -ψ ➝ ⊥ := Context.deduct! this;
+    replace : (insert (□(ψ ➝ □ψ)) ↑Γ₁) *⊢[𝓢] ψ := of_imply_complement_bot this;
+    replace : ↑Γ₁ *⊢[𝓢] □(ψ ➝ □ψ) ➝ ψ := Context.deduct! this;
+    replace : (□'↑Γ₁) *⊢[𝓢] □(□(ψ ➝ □ψ) ➝ ψ) := Context.nec! this;
+    replace : (□'↑Γ₁) *⊢[𝓢] ψ := axiomGrz! ⨀ this;
+    replace : (□'□'↑Γ₁) *⊢[𝓢] □ψ := Context.nec! this;
+    replace : (□'↑Γ₁) *⊢[𝓢] □ψ := Context.boxbox_in_context_to_box this;
+    replace : (□'□'□'⁻¹X.1) *⊢[𝓢] □ψ := Context.weakening! ?h₂ this;
+    replace : (□'□'⁻¹X) *⊢[𝓢] □ψ := Context.boxbox_in_context_to_box this;
+    replace : X *⊢[𝓢] □ψ := Context.weakening! ?h₃ this;
+    exact membership_iff (by grind) |>.mpr this;
+    case h₁ =>
+      intro ξ;
       simp only [Set.mem_union, Finset.mem_coe, Set.mem_insert_iff];
       rintro (hξ₁ | hξ₂);
       . have := hΓ₁ hξ₁; tauto;
       . have := hΓ₂ hξ₂;
         simp at this;
         tauto;
+    case h₂ =>
+      intro ξ hξ;
+      obtain ⟨ξ, hξ, rfl⟩ := hξ;
+      have : ξ ∈ □'□'⁻¹X.1 := hΓ₁ hξ;
+      obtain ⟨χ, hχ, rfl⟩ := Finset.LO.exists_of_mem_box this;
+      use □χ;
+      grind;
+    case h₃ =>
+      intro ξ hξ;
+      obtain ⟨ξ, hξ, rfl⟩ := hξ;
+      tauto;
 
 omit [Consistent 𝓢] in
 lemma truthlemma_lemma3 : 𝓢 ⊢ (φ ⋏ □(φ ➝ □φ)) ➝ □φ := by
@@ -191,17 +195,17 @@ lemma truthlemma {X : (miniCanonicalModel 𝓢 φ).World} (q_sub : ψ ∈ φ.sub
         . constructor;
           . intro χ _ hr₂;
             apply hY.1;
-            simpa;
+            simpa [Finset.LO.preboxItr, Finset.LO.boxItr]
           . apply imp_iff_not_or (b := X = Y) |>.mpr;
             left; push_neg;
             use (ψ ➝ □ψ);
             refine ⟨?_, ?_, ?_⟩;
-            . simp_all;
+            . simp_all [Finset.LO.preboxItr, Finset.LO.boxItr];
             . apply hY.2;
               simp;
             . by_contra hC;
               have : ↑X *⊢[𝓢] ψ := membership_iff (by grind) |>.mp w;
-              have : ↑X *⊢[𝓢] □(ψ ➝ □ψ) := membership_iff (by simp; right; assumption) |>.mp hC;
+              have : ↑X *⊢[𝓢] □(ψ ➝ □ψ) := membership_iff (by simp [Finset.LO.preboxItr]; grind) |>.mp hC;
               have : ↑X *⊢[𝓢] (ψ ⋏ □(ψ ➝ □ψ)) ➝ □ψ := Context.of! $ truthlemma_lemma3;
               have : ↑X *⊢[𝓢] □ψ := this ⨀ K!_intro (by assumption) (by assumption);
               have : □ψ ∈ X := membership_iff (by grind) |>.mpr this;
@@ -220,7 +224,7 @@ lemma truthlemma {X : (miniCanonicalModel 𝓢 φ).World} (q_sub : ψ ∈ φ.sub
     . intro h Y RXY;
       apply ih (by grind) |>.mpr;
       have : ↑Y *⊢[𝓢] □ψ ➝ ψ := Context.of! $ axiomT!;
-      have : ↑Y *⊢[𝓢] ψ := this ⨀ (membership_iff (by grind) |>.mp (RXY.1 ψ (by simp; grind) h));
+      have : ↑Y *⊢[𝓢] ψ := this ⨀ (membership_iff (by grind) |>.mp (RXY.1 ψ (by simp [Finset.LO.preboxItr]; grind) h));
       exact membership_iff (by grind) |>.mpr this;
 
 lemma complete_of_mem_miniCanonicalFrame
